define spec monad

iocy/FancyTraces2.fsti
@@ -1,5 +1,6 @@
 module FancyTraces2
 
+open FStar.Tactics
 open FStar.List.Tot
 
 val promise (e:Type u#a) (a:Type u#b) : Type u#(max a b)
@@ -7,48 +8,81 @@ val promise (e:Type u#a) (a:Type u#b) : Type u#(max a b)
 noeq
 type event (e: Type0) : Type u#1 =
 | Ev : e -> event e
-| EAsync : #b:Type0 -> pr:promise e b -> lt:atrace e -> event e
+| EAsync : #b:Type0 -> pr:promise e b -> r:b -> lt:atrace e -> event e
 | EAwait : #b:Type0 -> pr:promise e b -> event e
 and atrace e : Type u#1 = list (event e)
 
 type trace e = list e
 
 val suffix_of : atrace 'e -> atrace 'e -> Type0
-val lemma_suffix_of_reflexive : l:atrace 'e -> Lemma (suffix_of l l)
+val lemma_suffix_of_reflexive : l:atrace 'e -> Lemma (suffix_of l l) [SMTPat (suffix_of l l)]
+val lemma_suffix_of_transitive :
+  l1:atrace 'e -> l2:atrace 'e -> l3:atrace 'e ->
+  Lemma (suffix_of l1 l2 /\ suffix_of l2 l3 ==> suffix_of l1 l3)
+  [SMTPat (suffix_of l1 l2); SMTPat (suffix_of l2 l3); SMTPat (suffix_of l1 l3)]
 
 val parallel_traces (e:Type0) : Type u#1 (* promise_id -> atrace e *)
 
 val mem (pr:promise 'e 'a) (pts:parallel_traces 'e) : Type0
-val sel (pr:promise 'e 'a) (pts:(parallel_traces 'e){pr `mem` pts}) : atrace 'e
+val sel_lt (pr:promise 'e 'a) (pts:(parallel_traces 'e){pr `mem` pts}) : atrace 'e
+val sel_r (pr:promise 'e 'a) (pts:(parallel_traces 'e){pr `mem` pts}) : 'a
 
-val insert (pr:promise 'e 'a) (lt:atrace 'e) (pts:parallel_traces 'e) : parallel_traces 'e
 
 let ord #e (pts pts':parallel_traces e) =
   (forall a (x:promise e a). x `mem` pts ==> x `mem` pts') /\
-  (forall a (x:promise e a). x `mem` pts ==> (sel x pts' `suffix_of` sel x pts))
+  (forall a (x:promise e a). x `mem` pts ==> (sel_lt x pts' `suffix_of` sel_lt x pts))
 
-val size : atrace 'e -> nat
+let ord_reflexive #e (pts:parallel_traces e) : Lemma (ord pts pts) = ()
+let ord_transitive #e (pts pts' pts'':parallel_traces e) :
+  Lemma (ord pts pts' /\ ord pts' pts'' ==> ord pts pts'') = ()
 
-let rec closed_atrace (m:parallel_traces 'e) (tr:atrace 'e) : GTot Type0 (decreases (size tr)) =
-  match tr with
-  | [] -> True
-  | Ev _ :: tl ->
-    assume (size tl < size tr);
-    closed_atrace m tl
-  | EAwait #_ #b pr :: tl ->
-    assume (size tl < size tr);
-    pr `mem` m /\ closed_atrace m tl
-  | EAsync pr lt :: tl ->
-    assume (size lt < size tr);
-    assume (size (lt@tl) < size tr);
-    closed_atrace m lt /\ (** the new thread can await on existing promises *)
-    closed_atrace (insert pr lt m) (lt@tl) (** the parent thread can await on the promise of the kid
-                                               and promises returned/created by the kid *)
+val insert (r:'a) (lt:atrace 'e) (pts:parallel_traces 'e) : 
+  pr:(promise 'e 'a){~(pr `mem` pts)} 
+  & 
+  pts':(parallel_traces 'e){pts `ord` pts'} // /\ pr `mem` pts' /\ sel pr pts' == lt}
 
-val interleave_map
-  (pts: parallel_traces 'e)
-  (#_: squash (forall a (pr:promise 'e a). pr `mem` pts ==> closed_atrace pts (sel pr pts)))
-  : list (trace 'e)
+val await_pr (pr:promise 'e 'a) (pts:(parallel_traces 'e){pr `mem` pts}) : 
+  pts':(parallel_traces 'e){pts `ord` pts'}
+
+// val size : atrace 'e -> nat
+
+val closed_atrace (pts:parallel_traces 'e) (tr:atrace 'e) : GTot Type0 //(decreases (size tr))
+  // match tr with
+  // | [] -> True
+  // | Ev _ :: tl ->
+  //   assume (size tl < size tr);
+  //   closed_atrace m tl
+  // | EAwait #_ #b pr :: tl ->
+  //   assume (size tl < size tr);
+  //   pr `mem` m /\ closed_atrace m tl
+  // | EAsync pr lt :: tl ->
+  //   assume (size lt < size tr);
+  //   assume (size (lt@tl) < size tr);
+  //   closed_atrace m lt /\ (** the new thread can await on existing promises *)
+  //   closed_atrace (dsnd (insert pr lt m)) (lt@tl) (** the parent thread can await on the promise of the kid
+  //                                              and promises returned/created by the kid *)
+
+val closed_atrace_insert #e #a h (pts:parallel_traces e) (r:a) lt : 
+  Lemma 
+    (requires (closed_atrace pts (h@lt)))
+    (ensures (
+      let (| pr, pts' |) = insert r lt pts in
+      closed_atrace pts' (h @ [EAsync pr r lt])))
+
+val closed_atrace_await_pr #e #a (pr:promise e a) h pts :
+  Lemma 
+    (requires (closed_atrace pts h))
+    (ensures (closed_atrace (await_pr pr pts) (h @ [EAwait pr])))
+
+val closed_atrace_produce #e (ev:e) h pts :
+  Lemma 
+    (requires (closed_atrace pts h))
+    (ensures (closed_atrace pts (h @ [Ev ev])))
+
+// val interleave_map
+//   (pts: parallel_traces 'e)
+//   (#_: squash (forall a (pr:promise 'e a). pr `mem` pts ==> closed_atrace pts (sel pr pts)))
+//   : list (trace 'e)
 
 let w_pre e = h:atrace e -> pts:parallel_traces e{
   closed_atrace pts h
@@ -64,9 +98,54 @@ let w_post e a h pts =
 
 let w e a = h:atrace e -> pts:parallel_traces e{closed_atrace pts h} -> w_post e a h pts -> Type0
 
+let w' e a = s0:nat -> w e (nat * a)
+
 let encode_pre_post_in_w #e #a
   (pre:w_pre e)
   (post:(h:atrace e -> pts:parallel_traces e -> w_post e a h pts))
   : w e a
   = (fun h pts p -> pre h pts /\ (forall r' lt' pts'. post h pts r' lt' pts' ==> p r' lt' pts'))
+
+let w_return e #a (x:a) : w e a =
+  fun h pts p -> p x [] pts
+
+let w_bind #e #a #b (m:w e a) (f: a -> w e b) : w e b =
+  fun h pts post ->
+    m h pts (fun r' lt' pts' ->
+        f r' (h@lt') pts' (fun r'' lt'' pts'' ->
+        append_assoc h lt' lt'';
+        post r'' (lt'@lt'') pts''))
+
+let w_async #e #a (wf:w e a) : w e (promise e a) =
+  fun h pts post ->
+    wf h pts (fun r' lt' pts' ->
+      let (| pr, pts'' |) = insert r' lt' pts' in
+      closed_atrace_insert h pts' r' lt';
+      post pr [EAsync pr r' lt'] pts'')
+
+let w_await #e #a (pr:promise e a) : w e a =
+  fun h pts post ->
+    pr `mem` pts /\ 
+    (closed_atrace_await_pr pr h pts;
+    post (sel_r pr pts) [EAwait pr] (await_pr pr pts))
+
+let w_produce #e (ev:e) : w e unit =
+  fun h pts post ->
+    closed_atrace_produce ev h pts;
+    post () [Ev ev] pts
+
+
+let (let!) = w_bind
+
+let f (pr:promise int unit) : w int unit =
+  w_await pr ;!
+  w_produce 0
+
+let g () : w int unit =
+  let! pr' = w_async ( 
+    let! pr = w_async (w_produce (-2)) in
+    f pr) in (** h of f = [EAsync pr]) **)
+  let! pr'' = w_async (w_produce (-1)) in
+  w_await pr' ;!
+  w_await pr''
 
